Write conversions and add tests

arm/proofs/aes_xts_decrypt_spec.ml
@@ -8,37 +8,6 @@ let pp_print_num fmt tm =
   pp_print_string fmt (string_of_num_hex n) in
 install_user_printer("pp_print_num",pp_print_num);;
 
-(*
-IEEE Standard for Cryptographic Protection of
-Data on Block-Oriented Storage Devices
-https://ieeexplore.ieee.org/stamp/stamp.jsp?tp=&arnumber=8637988
-
-Section 5.4.1
-
-a) T ← AES-enc(Key2, i) ⊗ αj
-b) CC ← C ⊕ T
-c) PP ← AES-dec(Key1, CC)
-d) P ← PP ⊕ T
-
-*)
-
-let xts_init_tweak = new_definition
-  `xts_init_tweak (iv:int128) (key_schedule:int128 list) =
-    aes256_encrypt iv key_schedule`;;
-
-let aes256_xts_decrypt_round = new_definition
-  `aes256_xts_decrypt_round (C:int128) (tk:int128) (key_schedule:int128 list) =
-    let CC = word_xor C tk in
-    let PP = aes256_decrypt CC key_schedule in
-    word_xor PP tk`;;
-
-let aes256_xts_decrypt_1block = new_definition
-  `aes256_xts_decrypt_1block
-    (C:int128) (iv:int128) (key1:int128 list) (key2:int128 list) =
-    let tk = xts_init_tweak iv key2 in
-    aes256_xts_decrypt_round C tk key1`;;
-
-
 (* Test vector:
 key1:
 c70a951e84370d1836bdd387607e94e5
@@ -74,12 +43,40 @@ c26c685728b9a2356d1ecd82358affbf
 4d05c122ade7966a94e4658247817701
 21a29367e3cefb30cb775905a6699487
 
+1 block
 iv: 0000000000000000000000123456789a
-
 out: 88c87a8644e587dc7e3057edf2a80cc3
-
 in: 0f0e0d0c0b0a09080706050403020100
- *)
+
+1 block + 6 bytes
+iv: 0000000000000000000000123456789a
+out: 57edf2a80cc389a4b92cde579f93da9ae5cc8b18e875
+in: 1514131211100f0e0d0c0b0a0908070605040302010
+
+3 blocks + 3 bytes
+iv: 0000000000000000000000123456789a
+out: 41c2e1e4a22c106ace4c926e3725aa6877a4be5b7b62cb514595696240d72889208c3488c87a8644e587dc7e3057edf2a80cc3
+in: 3231302f2e2d2c2b2a292827262524232221201f1e1d1c1b1a191817161514131211100f0e0d0c0b0a09080706050403020100
+
+*)
+
+let ciphertext = new_definition
+  `ciphertext = [word 0xc3; word 0x0c; word 0xa8; word 0xf2
+  ; word 0xed; word 0x57; word 0x30; word 0x7e
+  ; word 0xdc; word 0x87; word 0xe5; word 0x44
+  ; word 0x86; word 0x7a; word 0xc8; word 0x88] : byte list`;;
+let iv_tweak = new_definition
+  `iv_tweak = (word 0x0000000000000000000000123456789a) : int128`;;
+let perror = new_definition
+  `perorr = [ word 0; word 0; word 0; word 0
+   ; word 0; word 0; word 0; word 0
+   ; word 0; word 0; word 0; word 0
+   ; word 0; word 0; word 0; word 0] : byte list`;;
+let plaintext = new_definition
+  `plaintext = [word 0x0f; word 0x0e; word 0x0d; word 0x0c
+   ; word 0x0b; word 0x0a; word 0x09; word 0x08
+   ; word 0x07; word 0x06; word 0x05; word 0x04
+   ; word 0x03; word 0x02; word 0x01; word 0x00] : byte list`;;
 
 let KEY1 = new_definition `KEY1:int128 list =
   [ word 0xc70a951e84370d1836bdd387607e94e5
@@ -117,19 +114,57 @@ let KEY2 = new_definition `KEY2:int128 list =
   ; word 0x21a29367e3cefb30cb775905a6699487
   ]`;;
 
+(*
+IEEE Standard for Cryptographic Protection of
+Data on Block-Oriented Storage Devices
+https://ieeexplore.ieee.org/stamp/stamp.jsp?tp=&arnumber=8637988
+
+Section 5.4.1
+
+a) T ← AES-enc(Key2, i) ⊗ αj
+b) CC ← C ⊕ T
+c) PP ← AES-dec(Key1, CC)
+d) P ← PP ⊕ T
+
+*)
+
+let xts_init_tweak = new_definition
+  `xts_init_tweak (iv:int128) (key_schedule:int128 list) =
+    aes256_encrypt iv key_schedule`;;
+
+let XTS_INIT_TWEAK_CONV =
+  REWR_CONV xts_init_tweak THENC AESENC_HELPER_CONV;;
+
+(REWRITE_CONV [iv_tweak;KEY2] THENC XTS_INIT_TWEAK_CONV) `xts_init_tweak iv_tweak KEY2`;;
+
+let aes256_xts_decrypt_round = new_definition
+  `aes256_xts_decrypt_round (C:int128) (tk:int128) (key_schedule:int128 list) =
+    let CC = word_xor C tk in
+    let PP = aes256_decrypt CC key_schedule in
+    word_xor PP tk`;;
+
+let AES256_XTS_DECRYPT_ROUND_CONV =
+  REWRITE_CONV [aes256_xts_decrypt_round] THENC
+  SUBLET_CONV WORD_RED_CONV THENC
+  let_CONV THENC
+  SUBLET_CONV AESDEC_HELPER_CONV THENC
+  let_CONV THENC WORD_RED_CONV;;
+
+(* (REWRITE_CONV [iv_tweak; KEY2] THENC AES256_XTS_DECRYPT_ROUND_CONV)
+  `aes256_xts_decrypt_round iv_tweak iv_tweak KEY2`;; *)
+
+let aes256_xts_decrypt_1block = new_definition
+  `aes256_xts_decrypt_1block
+    (C:int128) (iv:int128) (key1:int128 list) (key2:int128 list) =
+    let tk = xts_init_tweak iv key2 in
+    aes256_xts_decrypt_round C tk key1`;;
+
 let XTSDEC_1BLOCK_HELPER_CONV =
   REWR_CONV aes256_xts_decrypt_1block THENC
   REWRITE_CONV [xts_init_tweak] THENC
-  SUBLET_CONV (AESENC_HELPER_CONV KEY2) THENC
+  SUBLET_CONV AESENC_HELPER_CONV THENC
   let_CONV THENC
-  REWRITE_CONV [aes256_xts_decrypt_round] THENC
-  SUBLET_CONV (DEPTH_CONV (WORD_RED_CONV ORELSEC NUM_RED_CONV)) THENC
-  PRINT_TERM_CONV THENC
-  let_CONV THENC
-  SUBLET_CONV (AESDEC_HELPER_CONV KEY1) THENC
-  let_CONV THENC
-  DEPTH_CONV (WORD_RED_CONV ORELSEC NUM_RED_CONV)
-  ;;
+  AES256_XTS_DECRYPT_ROUND_CONV;;
 
 (*162 seconds
 time prove (`aes256_xts_decrypt_1block
@@ -138,21 +173,6 @@ time prove (`aes256_xts_decrypt_1block
   KEY1 KEY2 = word 0x0f0e0d0c0b0a09080706050403020100`,
   CONV_TAC(LAND_CONV XTSDEC_1BLOCK_HELPER_CONV) THEN REFL_TAC);;
 *)
-
-(* Compute not working, takes longer time than hand written conv *)
-needs "Library/words.ml";;
-let rw = Compute.bool_compset();;
-word_compute_add_convs rw;;
-num_compute_add_convs rw;;
-Compute.add_thms [aes256_xts_decrypt_1block;aes256_xts_decrypt_round;xts_init_tweak;
-  aes256_encrypt;KEY1;KEY2;EL_CONS;LET_END_DEF;aes256_decrypt;aes_sub_bytes;aes_inv_shift_rows;
-  aes256_decrypt_round] rw;;
-let my_conv = Compute.WEAK_CBV_CONV rw;;
-
-my_conv `aes256_xts_decrypt_1block
-  (word 0x88c87a8644e587dc7e3057edf2a80cc3)
-  (word 0x0000000000000000000000123456789a)
-  KEY1 KEY2`;;
 
 (*******************************************)
 (* AES-XTS decryption full *)
@@ -169,30 +189,52 @@ let bytes_to_int128 = define
   `bytes_to_int128 (bs : byte list) : int128 =
     word_join
       (word_join
-        (word_join (word_join (EL 7 bs) (EL 6 bs) : int16) (word_join (EL 5 bs) (EL 4 bs) : int16) : int32)
-        (word_join (word_join (EL 3 bs) (EL 2 bs) : int16) (word_join (EL 1 bs) (EL 8 bs) : int16) : int32) : int64)
+        (word_join (word_join (EL 15 bs) (EL 14 bs) : int16) (word_join (EL 13 bs) (EL 12 bs) : int16) : int32)
+        (word_join (word_join (EL 11 bs) (EL 10 bs) : int16) (word_join (EL 9 bs) (EL 8 bs) : int16) : int32) : int64)
       (word_join
         (word_join (word_join (EL 7 bs) (EL 6 bs) : int16) (word_join (EL 5 bs) (EL 4 bs) : int16) : int32)
         (word_join (word_join (EL 3 bs) (EL 2 bs) : int16) (word_join (EL 1 bs) (EL 0 bs) : int16) : int32) : int64)`;;
 
+let EL_16_8_CLAUSES =
+  let pat = `EL n [x0;x1;x2;x3;x4;x5;x6;x7;x8;x9;x10;x11;x12;x13;x14;x15]:byte` in
+  map (fun n -> EL_CONV(subst [mk_small_numeral n,`n:num`] pat)) (0--15);;
+
+let BYTES_TO_INT128_CONV =
+  REWRITE_CONV [bytes_to_int128] THENC
+  REWRITE_CONV EL_16_8_CLAUSES THENC
+  DEPTH_CONV WORD_RED_CONV;;
+
+BYTES_TO_INT128_CONV `bytes_to_int128
+    [word 0x0f; word 0x0e; word 0x0d; word 0x0c
+   ; word 0x0b; word 0x0a; word 0x09; word 0x08
+   ; word 0x07; word 0x06; word 0x05; word 0x04
+   ; word 0x03; word 0x02; word 0x01; word 0x00]`;;
+
 let int128_to_bytes = define
   `int128_to_bytes (w : int128) : byte list =
-    [word_subword w (0, 1);
-     word_subword w (1, 1);
-     word_subword w (2, 1);
-     word_subword w (3, 1);
-     word_subword w (4, 1);
-     word_subword w (5, 1);
-     word_subword w (6, 1);
-     word_subword w (7, 1);
-     word_subword w (8, 1);
-     word_subword w (9, 1);
-     word_subword w (10, 1);
-     word_subword w (11, 1);
-     word_subword w (12, 1);
-     word_subword w (13, 1);
-     word_subword w (14, 1);
-     word_subword w (15, 1)]`;;
+    [word_subword w (0, 8);
+     word_subword w (8, 8);
+     word_subword w (16, 8);
+     word_subword w (24, 8);
+     word_subword w (32, 8);
+     word_subword w (40, 8);
+     word_subword w (48, 8);
+     word_subword w (56, 8);
+     word_subword w (64, 8);
+     word_subword w (72, 8);
+     word_subword w (80, 8);
+     word_subword w (88, 8);
+     word_subword w (96, 8);
+     word_subword w (104, 8);
+     word_subword w (112, 8);
+     word_subword w (120, 8)]`;;
+
+let INT128_TO_BYTES_CONV =
+  REWRITE_CONV [int128_to_bytes] THENC
+  DEPTH_CONV WORD_RED_CONV;;
+
+INT128_TO_BYTES_CONV `int128_to_bytes (word 0x0102030405060708090a0b0c0d0e0f)`;;
+
 
 (* Multiplication by the primitive element \alpha in GF(2^128) *)
 let GF_128_mult_by_primitive = new_definition
@@ -202,27 +244,31 @@ let GF_128_mult_by_primitive = new_definition
     let mask = word_ishr tweak 127 in
     word_xor (word_and mask (word 0x87)) shifted`;;
 
-let FST3 = define
-  `FST3 (x:a#b#c) = FST x`;;
-let SND3 = define
-  `SND3 (x:a#b#c) = FST (SND x)`;;
-let THD3 = define
-  `THD3 (x:a#b#c) = SND (SND x)`;;
+let GF_128_MULT_BY_PRIMITIVE_CONV =
+  REWRITE_CONV [GF_128_mult_by_primitive] THENC
+  REPEATC let_CONV THENC
+  DEPTH_CONV WORD_RED_CONV;;
+
+GF_128_MULT_BY_PRIMITIVE_CONV `GF_128_mult_by_primitive (word 0xffffffffffffffffffffffffffffffff)`;;
+
+let FST3 = define `FST3 (x:a#b#c) = FST x`;;
+let SND3 = define `SND3 (x:a#b#c) = FST (SND x)`;;
+let THD3 = define `THD3 (x:a#b#c) = SND (SND x)`;;
 
 let eth = prove_general_recursive_function_exists
  `?aes256_xts_decrypt_rec.
-    ! (i:num) (m:num) (C:byte list) (iv:int128) (key1:int128 list) (key2:int128 list).
-    aes256_xts_decrypt_rec i m C iv key1 key2 : (byte list)#int128#num =
+    ! (i:num) (m:num) (C:byte list) (iv:int128) (key1:int128 list).
+    aes256_xts_decrypt_rec i m C iv key1 : (byte list)#int128#num =
     if m < i then ([], iv, i)
     else
       let current_block = bytes_to_int128 (SUB_LIST (i * 16, 16) C) in
       let curr = int128_to_bytes (aes256_xts_decrypt_round current_block iv key1) in
       let iv = GF_128_mult_by_primitive iv in
-      let res = aes256_xts_decrypt_rec (i + 1) m C iv key1 key2 in
+      let res = aes256_xts_decrypt_rec (i + 1) m C iv key1 in
       (APPEND curr (FST3 res), SND3 res, THD3 res)`;;
 
 let wfth = prove(hd(hyp eth),
-  EXISTS_TAC `MEASURE (\(i:num,m:num,C:byte list,iv:int128,key1:int128 list,key2:int128 list). (m + 1) - i)` THEN
+  EXISTS_TAC `MEASURE (\(i:num,m:num,C:byte list,iv:int128,key1:int128 list). (m + 1) - i)` THEN
   REWRITE_TAC[WF_MEASURE; MEASURE] THEN ARITH_TAC);;
 
 let exists_lemma = PROVE_HYP wfth eth;;
@@ -230,21 +276,68 @@ let exists_lemma = PROVE_HYP wfth eth;;
 (* Note: results are stored in LSByte to MSByte *)
 let aes256_xts_decrypt_rec = new_specification ["aes256_xts_decrypt_rec"] exists_lemma;;
 
+let rec AES256_XTS_DECRYPT_REC_CONV tm =
+  let BASE_CONV =
+    REWR_CONV aes256_xts_decrypt_rec THENC
+    DEPTH_CONV NUM_RED_CONV in
+  let INDUCT_CONV =
+    REWR_CONV aes256_xts_decrypt_rec THENC
+    DEPTH_CONV NUM_RED_CONV THENC
+    ONCE_DEPTH_CONV SUB_LIST_CONV THENC
+    ONCE_DEPTH_CONV BYTES_TO_INT128_CONV THENC let_CONV THENC
+    SUBLET_CONV (RAND_CONV AES256_XTS_DECRYPT_ROUND_CONV) THENC
+    SUBLET_CONV INT128_TO_BYTES_CONV THENC let_CONV THENC
+    SUBLET_CONV GF_128_MULT_BY_PRIMITIVE_CONV THENC let_CONV THENC
+    SUBLET_CONV AES256_XTS_DECRYPT_REC_CONV THENC let_CONV THENC
+    REWRITE_CONV [FST3;SND3;THD3;APPEND] in
+  match tm with
+  | Comb
+       (Comb
+         (Comb
+           (Comb
+             (Comb (Const ("aes256_xts_decrypt_rec", _), i), m),
+            _),
+          _),
+        _) ->
+    if dest_numeral m </ dest_numeral i
+    then BASE_CONV tm
+    else INDUCT_CONV tm
+  | _ -> failwith "AES256_XTS_DECRYPT_REC_CONV: inapplicable";;
+
+(REWRITE_CONV [iv_tweak;KEY1;KEY2;ciphertext] THENC AES256_XTS_DECRYPT_REC_CONV)
+  `aes256_xts_decrypt_rec 0 0 ciphertext iv_tweak KEY1`;;
+
 let cipher_stealing = new_definition
-  `cipher_stealing (block:byte list) (tail:byte list) (tail_len:num) (iv:int128) (key1:int128 list): (byte list)#(byte list) =
+  `cipher_stealing (block:byte list) (tail:byte list) (tail_len:num)
+    (iv:int128) (key1:int128 list): (byte list)#(byte list) =
     let iv_last = GF_128_mult_by_primitive iv in
     let PP = int128_to_bytes (aes256_xts_decrypt_round (bytes_to_int128 block) iv_last key1) in
-    let len = tail_len * 8 in
     let Pm = SUB_LIST (0, tail_len) PP in
     let CP = SUB_LIST (tail_len, 16 - tail_len) PP in
     let CC = bytes_to_int128 (APPEND tail CP) in
     let Pm1 = int128_to_bytes (aes256_xts_decrypt_round CC iv key1) in
     (Pm1, Pm)`;;
 
+let CIPHER_STEALING_CONV =
+  REWRITE_CONV [cipher_stealing] THENC
+  SUBLET_CONV GF_128_MULT_BY_PRIMITIVE_CONV THENC let_CONV THENC
+  SUBLET_CONV (ONCE_DEPTH_CONV BYTES_TO_INT128_CONV) THENC
+  SUBLET_CONV (RAND_CONV AES256_XTS_DECRYPT_ROUND_CONV) THENC
+  SUBLET_CONV INT128_TO_BYTES_CONV THENC let_CONV THENC
+  SUBLET_CONV SUB_LIST_CONV THENC let_CONV THENC
+  SUBLET_CONV (DEPTH_CONV NUM_RED_CONV) THENC (* For evaluating 16 - tail_len *)
+  SUBLET_CONV SUB_LIST_CONV THENC let_CONV THENC
+  SUBLET_CONV (ONCE_DEPTH_CONV (REWRITE_CONV [APPEND])) THENC
+  SUBLET_CONV BYTES_TO_INT128_CONV THENC let_CONV THENC
+  SUBLET_CONV (RAND_CONV AES256_XTS_DECRYPT_ROUND_CONV) THENC
+  SUBLET_CONV INT128_TO_BYTES_CONV THENC let_CONV;;
+
+(REWRITE_CONV [ciphertext;iv_tweak;KEY1] THENC CIPHER_STEALING_CONV)
+  `cipher_stealing ciphertext [(word 0x0)] 1 iv_tweak KEY1`;;
+
 (* Depending on the tail, either do one block decryption or do cipher stealing *)
 let aes256_xts_decrypt_tail = new_definition
-  `aes256_xts_decrypt_tail (i:num) (m:num) (tail_len:num) 
-    (C:byte list) (iv:int128) (key1:int128 list) (key2:int128 list) : byte list =
+  `aes256_xts_decrypt_tail (i:num) (tail_len:num) (C:byte list) (iv:int128) (key1:int128 list) : byte list =
     if tail_len = 0 then
       let Cm1 = bytes_to_int128 (SUB_LIST (i * 16, 16) C) in
       int128_to_bytes (aes256_xts_decrypt_round Cm1 iv key1)
@@ -254,6 +347,47 @@ let aes256_xts_decrypt_tail = new_definition
 
       let res_cs = cipher_stealing Cm1 Ctail tail_len iv key1 in
       APPEND (FST res_cs) (SND res_cs)`;;
+
+let AES256_XTS_DECRYPT_TAIL_CONV tm =
+  let ONE_BLOCK_CONV =
+    REWR_CONV aes256_xts_decrypt_tail THENC
+    DEPTH_CONV NUM_RED_CONV THENC
+    SUBLET_CONV (RAND_CONV SUB_LIST_CONV) THENC
+    SUBLET_CONV BYTES_TO_INT128_CONV THENC let_CONV THENC
+    RAND_CONV AES256_XTS_DECRYPT_ROUND_CONV THENC
+    INT128_TO_BYTES_CONV in
+  let ONE_BLOCK_AND_TAIL_CONV =
+    REWR_CONV aes256_xts_decrypt_tail THENC
+    DEPTH_CONV NUM_RED_CONV THENC
+    SUBLET_CONV SUB_LIST_CONV THENC let_CONV THENC
+    SUBLET_CONV SUB_LIST_CONV THENC let_CONV THENC
+    SUBLET_CONV CIPHER_STEALING_CONV THENC let_CONV THENC
+    REWRITE_CONV [FST;SND] THENC REWRITE_CONV [APPEND] in
+  match tm with
+  | Comb
+       (Comb
+         (Comb
+           (Comb
+             (Comb
+               (Const ("aes256_xts_decrypt_tail", _), _), tail_len),
+            _),
+          _),
+        _) ->
+    if dest_numeral tail_len =/ num 0
+    then ONE_BLOCK_CONV tm
+    else ONE_BLOCK_AND_TAIL_CONV tm
+  | _ -> failwith "AES256_XTS_DECRYPT_TAIL_CONV: inapplicable";;
+
+(REWRITE_CONV [ciphertext;iv_tweak;KEY1;KEY2] THENC AES256_XTS_DECRYPT_TAIL_CONV)
+  `aes256_xts_decrypt_tail 0 0 ciphertext iv_tweak KEY1`;;
+
+(REWRITE_CONV [iv_tweak;KEY1;KEY2] THENC AES256_XTS_DECRYPT_TAIL_CONV)
+`aes256_xts_decrypt_tail 0 1
+   [word 0xc3; word 0x0c; word 0xa8; word 0xf2
+  ; word 0xed; word 0x57; word 0x30; word 0x7e
+  ; word 0xdc; word 0x87; word 0xe5; word 0x44
+  ; word 0x86; word 0x7a; word 0xc8; word 0x88; word 0x00]
+  iv_tweak KEY1`;;
 
 (* The main decryption function *)
 (* Note: the specification does not handle the case of len < 16, which is
@@ -266,21 +400,21 @@ let aes256_xts_decrypt_tail = new_definition
    iv: Initialization vector (tweak) as an int128
    key1: Key schedule for AES-256 decryption
    key2: Key schedule for AES-256 encryption for the tweak
-   P_error: Error output plaintext in case of invalid input length
+   perror: Error output plaintext in case of invalid input length
 
    return: Output plaintext as a byte list
 
-   When input len < 16, the function returns P_error,
+   When input len < 16, the function returns perror,
    which will be the initial value stored in output address.
 *)
 (* TODO: Challenge lemma: proving that the output is of same length as input *)
-(* TODO: Double check if NIST spec talks about the error case len < 16 *)
+(* TODO: Double check if IEEE and NIST spec talks about the error case len < 16 *)
 (* TODO: Double check the pseudo code in the spec for tweak caculation in ANEX c *)
 let aes256_xts_decrypt = new_definition
   `aes256_xts_decrypt
-    (C:byte list) (len:num) (iv:int128) (key1:int128 list) (key2:int128 list) (P_error:byte list) : byte list =
+    (C:byte list) (len:num) (iv:int128) (key1:int128 list) (key2:int128 list) (perror:byte list) : byte list =
     if len < 16 then
-      P_error
+      perror
     else
       let tail = len MOD 16 in
       let m = (len - tail) DIV 16 in
@@ -288,37 +422,107 @@ let aes256_xts_decrypt = new_definition
 
       let iv = xts_init_tweak iv key2 in
       if m < 2 then
-        aes256_xts_decrypt_tail i m tail C iv key1 key2
+        aes256_xts_decrypt_tail i tail C iv key1
       else
-        let res = aes256_xts_decrypt_rec 0 (m - 2) C iv key1 key2 in
-        let Ptail = aes256_xts_decrypt_tail (THD3 res) m tail C (SND3 res) key1 key2 in
+        let res = aes256_xts_decrypt_rec 0 (m - 2) C iv key1 in
+        let Ptail = aes256_xts_decrypt_tail (THD3 res) tail C (SND3 res) key1 in
         APPEND (FST3 res) Ptail`;;
+
+let AES256_XTS_DECRYPT_CONV tm =
+  let ERROR_CONV =
+    REWR_CONV aes256_xts_decrypt THENC
+    DEPTH_CONV NUM_RED_CONV in
+  let MORE_THAN_2_CONV =
+    REWRITE_CONV [FST3;SND3;THD3] THENC
+    SUBLET_CONV AES256_XTS_DECRYPT_REC_CONV THENC let_CONV THENC
+    SUBLET_CONV AES256_XTS_DECRYPT_TAIL_CONV THENC let_CONV THENC
+    REWRITE_CONV [APPEND] in
+  let BODY_CONV =
+    REWR_CONV aes256_xts_decrypt THENC
+    DEPTH_CONV NUM_RED_CONV THENC let_CONV THENC
+    DEPTH_CONV NUM_RED_CONV THENC let_CONV THENC let_CONV THENC
+    SUBLET_CONV XTS_INIT_TWEAK_CONV THENC let_CONV THENC
+    DEPTH_CONV NUM_RED_CONV THENC
+    (AES256_XTS_DECRYPT_TAIL_CONV ORELSEC MORE_THAN_2_CONV) in
+  match tm with
+  | Comb
+   (Comb
+     (Comb
+       (Comb
+         (Comb
+           (Comb
+             (Const ("aes256_xts_decrypt", _), _), len),
+         _),
+       _),
+     _),
+   _) ->
+    if dest_numeral len </ num 16
+    then ERROR_CONV tm
+    else BODY_CONV tm
+  | _ -> failwith "AES256_XTS_DECRYPT_CONV: inapplicable";;
+
+
+(* TODO: figure out why perror isn't expanded out ??*)
+(REWRITE_CONV [perror] THENC AES256_XTS_DECRYPT_CONV)
+  `aes256_xts_decrypt ciphertext 5 iv_tweak KEY1 KEY2 perror`;;
+
+(REWRITE_CONV [ciphertext;iv_tweak;KEY1;KEY2;perror] THENC AES256_XTS_DECRYPT_CONV)
+  `aes256_xts_decrypt ciphertext 16 iv_tweak KEY1 KEY2 perror`;;
+
+(* 165 seconds *)
+time (REWRITE_CONV [iv_tweak;KEY1;KEY2;perror] THENC AES256_XTS_DECRYPT_CONV)
+  `aes256_xts_decrypt [word 0xc3; word 0x0c; word 0xa8; word 0xf2
+  ; word 0xed; word 0x57; word 0x30; word 0x7e
+  ; word 0xdc; word 0x87; word 0xe5; word 0x44
+  ; word 0x86; word 0x7a; word 0xc8; word 0x88
+  ; word 0xc3; word 0x0c; word 0xa8; word 0xf2
+  ; word 0xed; word 0x57; word 0x30; word 0x7e
+  ; word 0xdc; word 0x87; word 0xe5; word 0x44
+  ; word 0x86; word 0x7a; word 0xc8; word 0x88
+  ; word 0x00]
+  33 iv_tweak KEY1 KEY2 perror`;;
 
 (*******************************************)
 (* Conversions *)
 
-let ciphertext = new_definition
-  `[word 0xc3; word 0x0c; word 0xa8; word 0xf2
-  ; word 0xed; word 0x57; word 0x30; word 0x7e
-  ; word 0xdc; word 0x87; word 0xe5; word 0x44
-  ; word 0x86; word 0x7a; word 0xc8; word 0x88] : byte list`;;
-let iv = new_definition
-  `(word 0x0000000000000000000000123456789a) : int128`;;
-let P_error = new_definition
-  `[ word 0; word 0; word 0; word 0
-   ; word 0; word 0; word 0; word 0
-   ; word 0; word 0; word 0; word 0
-   ; word 0; word 0; word 0; word 0] : byte list`;;
-let plaintext = new_definition
-  `[word 0x0f; word 0x0e; word 0x0d; word 0x0c
-   ; word 0x0b; word 0x0a; word 0x09; word 0x08
-   ; word 0x07; word 0x06; word 0x05; word 0x04
-   ; word 0x03; word 0x02; word 0x01; word 0x00] : byte list`;;
+(*******************************************)
+(* Tests *)
 
-let rw = Compute.bool_compset();;
-word_compute_add_convs rw;;
-num_compute_add_convs rw;;
-Compute.add_thms [aes256_xts_decrypt;KEY1;KEY2;ciphertext;iv;P_error;plaintext] rw;;
-let my_conv = Compute.WEAK_CBV_CONV rw;;
+(* 1 block : 81 second *)
+time (REWRITE_CONV [iv_tweak;KEY1;KEY2;perror] THENC AES256_XTS_DECRYPT_CONV)
+  `aes256_xts_decrypt
+    [ word 0xc3; word 0x0c; word 0xa8; word 0xf2;
+      word 0xed; word 0x57; word 0x30; word 0x7e;
+      word 0xdc; word 0x87; word 0xe5; word 0x44;
+      word 0x86; word 0x7a; word 0xc8; word 0x88 ]
+    16 iv_tweak KEY1 KEY2 perror`;;
 
-my_conv `aes256_xts_decrypt C 16 iv KEY1 KEY2 P_error`;;
+(* 1 block + 6 bytes : 121 seconds *)
+time (REWRITE_CONV [iv_tweak;KEY1;KEY2;perror] THENC AES256_XTS_DECRYPT_CONV)
+  `aes256_xts_decrypt
+    [ word 0x75; word 0xe8; word 0x18; word 0x8b;
+      word 0xcc; word 0xe5; word 0x9a; word 0xda;
+      word 0x93; word 0x9f; word 0x57; word 0xde;
+      word 0x2c; word 0xb9; word 0xa4; word 0x89;eiifcbfhciurugujvrcfbnrlukjdrebhuklngddvufnf
+
+      word 0xc3; word 0x0c; word 0xa8; word 0xf2;
+      word 0xed; word 0x57 ]
+    22 iv_tweak KEY1 KEY2 perror`;;
+
+(* 3 blocks + 3 bytes : 206 seconds *)
+time (REWRITE_CONV [iv_tweak;KEY1;KEY2;perror] THENC AES256_XTS_DECRYPT_CONV)
+  `aes256_xts_decrypt
+    [ word 0xc3; word 0x0c; word 0xa8; word 0xf2;
+      word 0xed; word 0x57; word 0x30; word 0x7e;
+      word 0xdc; word 0x87; word 0xe5; word 0x44;
+      word 0x86; word 0x7a; word 0xc8; word 0x88;
+      word 0x34; word 0x8c; word 0x20; word 0x89;
+      word 0x28; word 0xd7; word 0x40; word 0x62;
+      word 0x69; word 0x95; word 0x45; word 0x51;
+      word 0xcb; word 0x62; word 0x7b; word 0x5b;
+      word 0xbe; word 0xa4; word 0x77; word 0x68;
+      word 0xaa; word 0x25; word 0x37; word 0x6e;
+      word 0x92; word 0x4c; word 0xce; word 0x6a;
+      word 0x10; word 0x2c; word 0xa2; word 0xe4;
+      word 0xe1; word 0xc2; word 0x41 ]
+    51 iv_tweak KEY1 KEY2 perror`;;
